language/move-prover/src/bytecode_translator.rs
@@ -1723,7 +1723,7 @@ impl<'env> ModuleTranslator<'env> {
                 );
                 emitln!(
                     self.writer,
-                    "$abort_code := i#$Integer({});",
+                    "$abort_code := i#$Integer({}) mod 256;",
                     str_local(*src)
                 );
                 emitln!(self.writer, "goto Abort;")
